Prop is now optional and removed from negfunext
Because x Bool can’t land into Prop.

src/config.v
@@ -18,7 +18,9 @@ Class Universes := {
   universesFlag : Type
 }.
 
-(* TODO: Class for Prop, or maybe even allow only one universe? *)
+Class WithProp := {
+  withpropFlag : Type
+}.
 
 Inductive Yes : Type := yes.
 Inductive No : Type := .
