src/checking_tactics.v
@@ -13,6 +13,7 @@ Context `{configReflection : config.Reflection}.
 Context `{configSimpleProducts : config.SimpleProducts}.
 Context `{configProdEta : config.ProdEta}.
 Context `{ConfigUniverses : config.Universes}.
+Context `{ConfigWithProp : config.WithProp}.
 
 (* Some tactic to compose substitutions. *)
 Lemma eqtype_subst_left :
@@ -133,6 +134,7 @@ Context `{configReflection : config.Reflection}.
 Context `{configSimpleProducts : config.SimpleProducts}.
 Context `{configProdEta : config.ProdEta}.
 Context `{ConfigUniverses : config.Universes}.
+Context `{ConfigWithProp : config.WithProp}.
 
 Lemma EqCompZero :
   forall {G D A u sbs},
@@ -1180,6 +1182,7 @@ Context `{configReflection : config.Reflection}.
 Context `{configSimpleProducts : config.SimpleProducts}.
 Context `{configProdEta : config.ProdEta}.
 Context `{ConfigUniverses : config.Universes}.
+Context `{ConfigWithProp : config.WithProp}.
 
 (* A lemma to do ZeroShift shifted, it not very robust as we would need
    some ZeroShift3 if ever we add a constructor that has three variables. *)
