src/ett.v
@@ -8,6 +8,7 @@ Context `{configReflection : config.Reflection}.
 Context `{configSimpleProducts : config.SimpleProducts}.
 Context `{ConfigProdEta : config.ProdEta}.
 Context `{ConfigUniverses : config.Universes}.
+Context `{ConfigWithProp : config.WithProp}.
 
 Definition isctx := isctx.
 Definition issubst := issubst.
