src/ett2ptt.v
@@ -11,6 +11,7 @@ Context `{configReflection : config.Reflection}.
 Context `{configSimpleProducts : config.SimpleProducts}.
 Context `{ConfigProdEta : config.ProdEta}.
 Context `{ConfigUniverses : config.Universes}.
+Context `{ConfigWithProp : config.WithProp}.
 
 (* Renaming ptt_sanity lemmata for readability. *)
 Definition ptt_sane_issubst := ptt_sanity.sane_issubst.
