src/inversion.v
@@ -19,6 +19,7 @@ Context `{configReflection : config.Reflection}.
 Context `{configSimpleProducts : config.SimpleProducts}.
 Context `{configProdEta : config.ProdEta}.
 Context `{ConfigUniverses : config.Universes}.
+Context `{ConfigWithProp : config.WithProp}.
 
 Fixpoint TermAbsInversion {G A B u T}
          (H : ptt.isterm G (lam A B u) T) {struct H} :
