src/ptt_inversion.v
@@ -13,6 +13,7 @@ Context `{ConfigReflection : config.Reflection}.
 Context `{configSimpleProducts : config.SimpleProducts}.
 Context `{configProdEta : config.ProdEta}.
 Context `{ConfigUniverses : config.Universes}.
+Context `{ConfigWithProp : config.WithProp}.
 
 Definition CtxExtendInversion G A (H : isctx (ctxextend G A)) :
   isctx G * istype G A.
